more (incl. sorry)

thys/Partitioned_Trace.thy
@@ -36,6 +36,19 @@ lemma in_mapM_set_iff: "xs \<in> mapM_set f ys \<longleftrightarrow> list_all2 (
 lemma mapM_set_mono: "f \<le> f' \<Longrightarrow> mapM_set f \<le> mapM_set f'"
   by (fastforce simp: le_fun_def in_mapM_set_iff elim!: list.rel_mono_strong)
 
+lemma mapM_set_determ: "mapM_set (determ f) = determ (map f)"
+  by (auto simp: fun_eq_iff in_mapM_set_iff list.rel_map list.rel_map(2)[where g=f, symmetric]
+      list.rel_eq intro!: list.rel_refl)
+
+lemma kleisli_mapM_set: "mapM_set f \<circ>\<then> mapM_set g = mapM_set (f \<circ>\<then> g)"
+  apply (auto simp: fun_eq_iff kleisli_set_def in_mapM_set_iff elim!: list_all2_trans[rotated])
+  apply (simp add: Bex_def in_mapM_set_iff relcompp_apply)
+  apply (insert list.rel_compp[where R="(\<lambda>x y. x \<in> f y)\<inverse>\<inverse>" and S="(\<lambda>x y. x \<in> g y)\<inverse>\<inverse>"])
+  apply (simp add: relcompp_apply[abs_def] list.rel_flip fun_eq_iff)
+  apply (drule spec)+
+  apply (erule iffD1)
+  by (simp add: list_all2_conv_all_nth)
+
 
 record 'a itsdb =
   db :: "'a set"
@@ -570,12 +583,12 @@ lemma w\<beta>_mwproject_mwhd: "w\<beta> (mwproject (origin (mwhd \<sigma>)) \<s
 lemma Least_less_Least: "\<exists>x::'a::wellorder. Q x \<Longrightarrow> (\<And>x. Q x \<Longrightarrow> \<exists>y. P y \<and> y < x) \<Longrightarrow> Least P < Least Q"
   by (metis LeastI2 less_le_trans not_le_imp_less not_less_Least)
 
-lemma sincreasing_ex_greater: "sincreasing s \<Longrightarrow> \<exists>i. (x::nat) < s !! i"
+lemma sincreasing_ex_greater: "sincreasing s \<Longrightarrow> \<exists>i\<ge>j. (x::nat) < s !! i"
   unfolding sincreasing_def
   apply (induction x)
    apply simp_all
-  using gr_implies_not0 apply blast
-  using Suc_lessI by fastforce
+   apply (meson dual_order.strict_implies_order less_eq_nat.simps(1) order.strict_trans1)
+  by (meson less_trans_Suc order.order_iff_strict order.trans)
 
 lemma infinitely_exists: "infinitely P s \<Longrightarrow> \<exists>i. P (s !! i)"
   by (auto simp: infinitely_def)
@@ -637,7 +650,7 @@ lemma reorder_termination: "fst (reorder_step st) = [] \<Longrightarrow>
 
     have 1: "wmarks (reorder_update ?x st) = DAList.update (origin ?x) (wmark ?x) (wmarks st)"
       by (simp add: reorder_update_def)
-    then have wmarks_st': "wmarks st' = ..."
+    then have wmarks_st': "wmarks st' = \<dots>"
       using step_eq by (auto simp: reorder_flush_def Let_def)
     then have "keyset (wmarks st') = mworigins \<sigma>"
       using \<open>keyset (wmarks st) = mworigins \<sigma>\<close>
@@ -693,7 +706,7 @@ lemma reorder_termination: "fst (reorder_step st) = [] \<Longrightarrow>
       note next_st'
       also have "next_to_emit st \<sigma> < the (DAList.lookup (wmarks st) k)"
         using 0 by (simp add: next_to_release_def split: if_splits)
-      also have "... \<le> the (DAList.lookup (wmarks st') k)"
+      also have "\<dots> \<le> the (DAList.lookup (wmarks st') k)"
         by (clarsimp simp: wmarks_st' lookup_update
             intro!: w\<beta>_inv[THEN bspec[of _ _ "origin (mwhd \<sigma>)"], OF origin_mwhd, THEN spec[of _ 0],
               simplified w\<beta>_mwproject_mwhd])
@@ -736,19 +749,416 @@ lemma reorder_termination: "fst (reorder_step st) = [] \<Longrightarrow>
   qed
   done
 
-corecursive reorder' :: "'a reorder_state \<Rightarrow> ('a set \<times> nat) stream" where
-  "reorder' st = (let (xs, st') = reorder_step st in
+corecursive reorder :: "'a reorder_state \<Rightarrow> ('a set \<times> nat) stream" where
+  "reorder st = (let (xs, st') = reorder_step st in
     case xs of
-      [] \<Rightarrow> reorder' st'
-    | x # xs' \<Rightarrow> x ## xs' @- reorder' st')"
+      [] \<Rightarrow> reorder st'
+    | x # xs' \<Rightarrow> x ## xs' @- reorder st')"
   by (relation "measure reorder_variant") (simp_all add: reorder_termination)
 
-lift_definition init_reorder_state :: "'a mwtrace \<Rightarrow> 'a reorder_state" is
-  "\<lambda>\<sigma>. (\<lparr>wmarks = Finite_Set.fold (\<lambda>k. DAList.update k 0) DAList.empty (mworigins \<sigma>),
-    buffer = DAList.empty\<rparr>, \<sigma>)"
-  sorry
+lift_definition init_alist :: "'a::linorder set \<Rightarrow> 'b \<Rightarrow> ('a, 'b) alist" is
+  "\<lambda>K v. if finite K then map (\<lambda>k. (k, v)) (sorted_list_of_set K) else []"
+  by (simp cong: map_cong)
 
-lift_definition reorder :: "'a mwtrace \<Rightarrow> 'a trace" is "\<lambda>\<sigma>. reorder' (init_reorder_state \<sigma>)"
-  sorry
+lemma keyset_init_alist: "finite K \<Longrightarrow> keyset (init_alist K v) = K"
+  by transfer (simp add: image_image)
+
+lemma lookup_init_alist: "finite K \<Longrightarrow> k \<in> K \<Longrightarrow> DAList.lookup (init_alist K v) k = Some v"
+  by transfer (simp add: map_of_map_restrict)
+
+lift_definition init_reorder_state :: "'a mwtrace \<Rightarrow> 'a reorder_state" is
+  "\<lambda>\<sigma>. (\<lparr>wmarks = init_alist (mworigins \<sigma>) 0, buffer = DAList.empty\<rparr>, \<sigma>)"
+  by (simp add: keyset_init_alist lookup_init_alist)
+
+definition reorder' :: "'a mwtrace \<Rightarrow> ('a set \<times> nat) stream" where
+  "reorder' \<sigma> = reorder (init_reorder_state \<sigma>)"
+
+
+definition least_idx :: "'a mwtrace \<Rightarrow> nat \<Rightarrow> nat" where
+  "least_idx \<sigma> i0 = (LEAST i. i0 \<le> i \<and> (\<exists>j. i = idx (mwnth \<sigma> j)))"
+
+definition idx_stream :: "'a mwtrace \<Rightarrow> nat stream" where
+  "idx_stream \<sigma> = siterate (least_idx \<sigma> \<circ> Suc) (least_idx \<sigma> 0)"
+
+definition collapse_idx :: "'a mwtrace \<Rightarrow> nat \<Rightarrow> 'a set" where
+  "collapse_idx \<sigma> i = (\<Union>{d. \<exists>j. i = idx (mwnth \<sigma> j) \<and> d = db (mwnth \<sigma> j)})"
+
+definition ts_of_idx :: "'a mwtrace \<Rightarrow> nat \<Rightarrow> nat" where
+  "ts_of_idx \<sigma> i = ts (mwnth \<sigma> (LEAST j. i = idx (mwnth \<sigma> j)))"
+
+definition reorder_alt :: "'a mwtrace \<Rightarrow> ('a set \<times> nat) stream" where
+  "reorder_alt \<sigma> = smap (\<lambda>i. (collapse_idx \<sigma> i, ts_of_idx \<sigma> i)) (idx_stream \<sigma>)"
+
+definition collapse_reorder_state :: "'a raw_reorder_state \<Rightarrow> 'a mwtrace \<Rightarrow>  (nat \<times> 'a set \<times> nat) set" where
+  "collapse_reorder_state st \<sigma>' =
+    {(i, (d \<union> (collapse_idx \<sigma>' i), t)) | i d t. (i, (d, t)) \<in> set (DAList.impl_of (buffer st))} \<union>
+    {(i, (collapse_idx \<sigma>' i, ts_of_idx \<sigma>' i)) | i. i \<notin> keyset (buffer st) \<and> (\<exists>j. i = idx (mwnth \<sigma>' j))}"
+
+lift_definition reorder_state_rel :: "'a mwtrace \<Rightarrow> 'a reorder_state \<Rightarrow> nat \<Rightarrow> bool" is
+  "\<lambda>\<sigma> (st, \<sigma>') n. collapse_reorder_state st \<sigma>' = {(i, collapse_idx \<sigma> i, ts_of_idx \<sigma> i) | i. i \<in> sset (sdrop n (idx_stream \<sigma>))}" .
+
+lemma ex_idx_ge: "\<exists>x\<ge>y. \<exists>j. x = idx (mwnth \<sigma> j)"
+  apply (transfer fixing: y)
+  subgoal for \<sigma>
+    apply (clarsimp simp: wtracep_def)
+    apply (drule bspec[where x="shd \<sigma>"])
+     apply (simp add: shd_sset)
+    apply clarify
+    apply (drule sincreasing_ex_greater[where x=y])
+    apply (thin_tac "\<forall>i j. _ i j")
+    apply clarsimp
+    subgoal for i
+      apply (drule spec)+
+      apply (drule mp)
+       apply (rule lessI[of i])
+      apply (drule (1) order.strict_trans2)
+      by (metis order.order_iff_strict snth_sfilter)
+    done
+  done
+
+lemma sset_idx_stream: "sset (idx_stream \<sigma>) = {i. \<exists>j. i = idx (mwnth \<sigma> j)}"
+  apply (auto simp: idx_stream_def sset_siterate)
+  subgoal for n
+    apply (induction n)
+     apply (simp add: least_idx_def)
+     apply (rule LeastI)
+     apply blast
+    apply clarsimp
+    subgoal for n j
+    apply (thin_tac _)
+    apply (simp add: least_idx_def)
+      apply (insert LeastI_ex[where P="\<lambda>i. Suc (idx (mwnth \<sigma> j)) \<le> i \<and> (\<exists>j. i = idx (mwnth \<sigma> j))"])
+      apply (drule meta_mp)
+      apply (rule ex_idx_ge)
+      apply simp
+      done
+    done
+  subgoal for j proof -
+    have "\<And>i'. i' \<le> i \<Longrightarrow> \<exists>j. i' = idx (mwnth \<sigma> j) \<Longrightarrow>
+      \<exists>n. i' = ((least_idx \<sigma> \<circ> Suc) ^^ n) (least_idx \<sigma> 0)" for i
+      apply (induction i)
+       apply (auto simp: least_idx_def intro!: exI[where x=0])[]
+      subgoal for i i'
+        apply (cases "i' = Suc i"; simp)
+        apply (cases "\<exists>i''. i'' \<le> i \<and> (\<exists>j. i'' = idx (mwnth \<sigma> j))")
+        subgoal
+          apply clarsimp
+          apply (drule meta_spec[where x="GREATEST i''. i'' \<le> i \<and> (\<exists>j. i'' = idx (mwnth \<sigma> j))"])
+          apply (drule meta_mp)
+           apply (metis (mono_tags, lifting) GreatestI_ex_nat)
+          apply (drule meta_mp)
+           apply (smt GreatestI_ex_nat)
+          apply clarify
+          subgoal for j j' n
+            apply (rule exI[where x="Suc n"])
+            apply (clarsimp simp: least_idx_def)
+            apply (rule Least_equality[symmetric])
+             apply (smt GreatestI_nat not_less_eq_eq)
+            by (metis (mono_tags, lifting) Greatest_le_nat not_less_eq_eq)
+          done
+        subgoal
+          apply (rule exI[where x=0])
+          apply (auto simp: least_idx_def)
+          by (smt Least_equality less_Suc_eq_le not_less)
+        done
+      done
+    then show ?thesis by auto
+  qed
+  done
+
+lemma reorder_state_rel_init: "reorder_state_rel \<sigma> (init_reorder_state \<sigma>) 0"
+  by transfer (simp add: collapse_reorder_state_def DAList.empty.rep_eq sset_idx_stream)
+
+lemma set_map_default: "set (DAList.impl_of (DAList.map_default k v f al)) =
+  {case DAList.lookup al k of None \<Rightarrow> (k, v) | Some v' \<Rightarrow> (k, f v')} \<union>
+  {x. x \<in> set (DAList.impl_of al) \<and> fst x \<noteq> k}"
+  apply (transfer fixing: k v f)
+  subgoal for xs by (induction xs) (auto simp: image_iff)
+  done
+
+lemma lookup_None_set_conv: "DAList.lookup al k = None \<longleftrightarrow> k \<notin> fst ` set (DAList.impl_of al)"
+  by (transfer fixing: k) (simp add: map_of_eq_None_iff)
+
+lemma lookup_Some_set_conv: "DAList.lookup al k = Some v \<longleftrightarrow> (k, v) \<in> set (DAList.impl_of al)"
+  by (transfer fixing: k v) simp
+
+lemma collapse_idx_mwtl: "collapse_idx \<sigma> i =
+  (if i = idx (mwhd \<sigma>) then db (mwhd \<sigma>) \<union> collapse_idx (mwtl \<sigma>) i else collapse_idx (mwtl \<sigma>) i)"
+  apply (auto simp: collapse_idx_def)
+      apply (metis mwnth_Suc mwnth_zero not0_implies_Suc)
+     apply (metis mwnth_zero)
+    apply (metis mwnth_Suc)
+   apply (metis mwnth_Suc mwnth_zero not0_implies_Suc)
+  apply (metis mwnth_Suc)
+  done
+
+lemma ts_of_idx_mwtl: "(\<exists>j. i = idx (mwnth \<sigma> j)) \<Longrightarrow> ts_of_idx \<sigma> i =
+  (if i = idx (mwhd \<sigma>) then ts (mwhd \<sigma>) else ts_of_idx (mwtl \<sigma>) i)"
+  apply (auto simp: ts_of_idx_def mwnth_zero)
+  apply (subgoal_tac "(LEAST j. i = idx (mwnth \<sigma> j)) = Suc (LEAST j. i = idx (mwnth (mwtl \<sigma>) j))")
+   apply (simp add: mwnth_Suc)
+  apply simp
+  apply (subst mwnth_Suc[symmetric])
+  apply (rule Least_Suc[OF refl])
+  apply (simp add: mwnth_zero)
+  done
+
+lemma alist_eq_key_imp_eq: "(k, v) \<in> set (DAList.impl_of al) \<Longrightarrow> (k, v') \<in> set (DAList.impl_of al) \<Longrightarrow> v = v'"
+  by (transfer fixing: k v v') (simp add: eq_key_imp_eq_value)
+
+lemma reorder_state_rel_step: "reorder_state_rel \<sigma> st n \<Longrightarrow>
+  reorder_step st = (xs, st') \<Longrightarrow> xs = stake (length xs) (sdrop n (reorder_alt \<sigma>)) \<and>
+    reorder_state_rel \<sigma> st' (n + length xs)"
+  apply (transfer fixing: \<sigma> n xs)
+  apply (clarsimp split: prod.splits)
+  subgoal premises assms for st \<sigma>' st'
+  proof -
+    note old_state = \<open>collapse_reorder_state st \<sigma>' =
+      {(i, collapse_idx \<sigma> i, ts_of_idx \<sigma> i) |i. i \<in> sset (sdrop n (idx_stream \<sigma>))}\<close>
+    note step_eq = \<open>_ = (xs, st')\<close>
+    let ?x = "mwhd \<sigma>'"
+    let ?st1 = "reorder_update ?x st"
+
+    have buffer_st1: "buffer ?st1 =
+      DAList.map_default (idx ?x) (db ?x, ts ?x) (\<lambda>(d, t). (d \<union> db ?x, t)) (buffer st)"
+      by (simp add: reorder_update_def)
+
+    have 1: "{(i, collapse_idx \<sigma>' i, ts_of_idx \<sigma>' i) |i. i \<notin> keyset (buffer st) \<and> (\<exists>j. i = idx (mwnth \<sigma>' j))} =
+      {(i, collapse_idx \<sigma>' i, if i = idx (mwhd \<sigma>') then ts (mwhd \<sigma>') else ts_of_idx (mwtl \<sigma>') i) |
+        i. i \<notin> keyset (buffer st) \<and> (\<exists>j. i = idx (mwnth \<sigma>' j))}"
+      by (simp only: ts_of_idx_mwtl cong: rev_conj_cong)
+    have 2: "(\<exists>j. i = idx (mwnth \<sigma>' j)) \<longleftrightarrow> i = idx (mwhd \<sigma>') \<or> (\<exists>j. i = idx (mwnth (mwtl \<sigma>') j))" for i
+      apply safe
+        apply (metis nat.exhaust mwnth_zero mwnth_Suc)
+       apply (metis mwnth_zero)
+      apply (metis mwnth_Suc)
+      done
+
+    have "collapse_reorder_state ?st1 (mwtl \<sigma>') = collapse_reorder_state st \<sigma>'"
+      unfolding collapse_reorder_state_def buffer_st1 set_map_default keyset_map_default 1
+      apply (subst (3 4) collapse_idx_mwtl)
+      unfolding 2 keyset.rep_eq
+      by (auto simp: lookup_None_set_conv lookup_Some_set_conv fst_eq_Domain Domain.simps
+          split: option.split dest: alist_eq_key_imp_eq)
+
+    show ?thesis sorry (* TODO *)
+  qed
+  done
+
+lemma reorder_eq_alt: "reorder_state_rel \<sigma> st n \<Longrightarrow> reorder st = sdrop n (reorder_alt \<sigma>)"
+  apply (coinduction arbitrary: st \<sigma> n rule: reorder.coinduct)
+  subgoal for st \<sigma> n
+    apply (induction st rule: reorder.inner_induct)
+    subgoal premises ind for st
+      apply (cases "fst (reorder_step st)")
+      subgoal
+        apply (frule ind(1))
+         apply (rule reorder_state_rel_step[where xs="[]", simplified, OF ind(2)])
+         apply (auto intro: prod_eqI)[]
+        apply (subst (1 3) reorder.code)
+        apply (simp add: split_beta)
+        done
+      subgoal for x xs
+        apply (insert reorder_state_rel_step[where xs="x # xs" and st'="snd (reorder_step st)", OF ind(2)])
+        apply (drule meta_mp)
+         apply (auto intro: prod_eqI)[]
+        apply (subst (1 3) reorder.code)
+        apply (clarsimp simp: split_beta)
+        apply (subst stake_sdrop[where n="length xs" and s="sdrop n (stl (reorder_alt \<sigma>))", symmetric])
+        apply (erule shift.friend.cong_shift)
+        apply (force intro: reorder.cong_base)
+        done
+      done
+    done
+  done
+
+lemma reorder'_eq_alt: "reorder' = reorder_alt"
+  using reorder_eq_alt[OF reorder_state_rel_init] by (auto simp: reorder'_def fun_eq_iff)
+
+
+locale wtrace_partition =
+  fixes \<sigma> :: "'a itrace" and n :: nat and ps :: "'a wtrace list"
+  assumes
+    n_greater_0: "n > 0" and
+    length_ps_eq_n: "length ps = n" and
+    sound_partition: "\<forall>k<n. \<forall>j. \<exists>i. w\<iota> (ps ! k) j = i\<iota> \<sigma> i \<and> w\<tau> (ps ! k) j = i\<tau> \<sigma> i \<and> w\<Gamma> (ps ! k) j \<subseteq> i\<Gamma> \<sigma> i" and
+    complete_partition1: "\<forall>i. \<exists>k<n. \<exists>j. w\<iota> (ps ! k) j = i\<iota> \<sigma> i \<and> w\<tau> (ps ! k) j = i\<tau> \<sigma> i" and
+    complete_partition2: "\<forall>i. \<forall>f \<in> i\<Gamma> \<sigma> i. \<exists>k<n. \<exists>j. w\<iota> (ps ! k) j = i\<iota> \<sigma> i \<and> w\<tau> (ps ! k) j = i\<tau> \<sigma> i \<and> f \<in> w\<Gamma> (ps ! k) j"
+
+definition wpartition :: "nat \<Rightarrow> 'a itrace \<Rightarrow> 'a wtrace list set" where
+  "wpartition n \<sigma> = {ps. wtrace_partition \<sigma> n ps}"
+
+definition least_w\<iota> :: "'a wtrace \<Rightarrow> nat \<Rightarrow> nat" where
+  "least_w\<iota> \<sigma> i0 = (LEAST i. i0 \<le> i \<and> (\<exists>j. i = w\<iota> \<sigma> j))"
+
+definition w\<iota>_stream :: "'a wtrace \<Rightarrow> nat stream" where
+  "w\<iota>_stream \<sigma> = siterate (least_w\<iota> \<sigma> \<circ> Suc) (least_w\<iota> \<sigma> 0)"
+
+definition collapse_w :: "'a wtrace \<Rightarrow> nat \<Rightarrow> 'a set" where
+  "collapse_w \<sigma> i = (\<Union>{d. \<exists>j. i = w\<iota> \<sigma> j \<and> d = w\<Gamma> \<sigma> j})"
+
+definition ts_of_w :: "'a wtrace \<Rightarrow> nat \<Rightarrow> nat" where
+  "ts_of_w \<sigma> i = w\<tau> \<sigma> (LEAST j. i = w\<iota> \<sigma> j)"
+
+lemma ex_w\<iota>_ge: "\<exists>x\<ge>i. \<exists>j. x = w\<iota> \<sigma> j"
+  apply (transfer fixing: i)
+  apply (clarsimp simp: wtracep_def)
+  apply (drule sincreasing_ex_greater[where j=0 and x=i])
+  by (metis gt_ex le_trans less_imp_le_nat smap_alt)
+
+lemma le_least_w\<iota>: "i \<le> least_w\<iota> \<sigma> i"
+  unfolding least_w\<iota>_def
+  apply (subgoal_tac "i \<le> (LEAST x. i \<le> x \<and> (\<exists>j. x = w\<iota> \<sigma> j)) \<and>
+          (\<exists>j. (LEAST x. i \<le> x \<and> (\<exists>j. x = w\<iota> \<sigma> j)) = w\<iota> \<sigma> j)")
+   apply (erule conjunct1)
+  apply (rule LeastI_ex)
+  by (rule ex_w\<iota>_ge)
+
+lemma ssorted_w\<iota>_stream: "ssorted (w\<iota>_stream \<sigma>)"
+  by (auto simp: w\<iota>_stream_def intro!: ssorted_siterate order_trans[OF _ le_least_w\<iota>])
+
+lemma sincreasing_w\<iota>_stream: "sincreasing (w\<iota>_stream \<sigma>)"
+  by (auto simp: w\<iota>_stream_def intro!: sincreasing_siterate order.strict_trans2[OF _ le_least_w\<iota>])
+
+lemma mono_ts_of_w: "i \<le> j \<Longrightarrow> \<exists>k. i = w\<iota> \<sigma> k \<Longrightarrow> \<exists>k. j = w\<iota> \<sigma> k \<Longrightarrow> ts_of_w \<sigma> i \<le> ts_of_w \<sigma> j"
+  unfolding ts_of_w_def
+  apply (transfer fixing: i j)
+  subgoal for \<sigma>
+    apply (clarsimp simp: wtracep_def)
+    apply (drule spec2[where P="\<lambda>i j. _ i j \<longrightarrow> ts (_ i) \<le> _ j"])
+    apply (erule mp)
+    by (metis (mono_tags, lifting) LeastI)
+  done
+
+lemma ex_snth_w\<iota>_stream: "\<exists>k. w\<iota>_stream \<sigma> !! i = w\<iota> \<sigma> k"
+  apply (induction i)
+   apply (auto simp add: w\<iota>_stream_def least_w\<iota>_def simp del: snth.simps intro: LeastI)
+  subgoal for i k
+    apply (insert LeastI_ex[where P="\<lambda>i. Suc (w\<iota> \<sigma> k) \<le> i \<and> (\<exists>j. i = w\<iota> \<sigma> j)"])
+    apply (drule meta_mp)
+     apply (rule ex_w\<iota>_ge)
+    apply (erule conjunct2)
+    done
+  done
+
+lemma le_w\<iota>_le_w\<tau>: "w\<iota> \<sigma> i \<le> w\<iota> \<sigma> j \<Longrightarrow> w\<tau> \<sigma> i \<le> w\<tau> \<sigma> j"
+  by transfer (simp add: wtracep_def)
+
+lemma w\<tau>_increasing: "\<exists>j>i. w\<tau> \<sigma> i < w\<tau> \<sigma> j"
+  by transfer (simp add: wtracep_def sincreasing_def)
+
+lift_definition reorder_w :: "'a wtrace \<Rightarrow> 'a itrace" is
+  "\<lambda>\<sigma>. smap (\<lambda>i. \<lparr>db=collapse_w \<sigma> i, ts=ts_of_w \<sigma> i, idx=i\<rparr>) (w\<iota>_stream \<sigma>)"
+  apply (simp add: stream.map_comp stream.map_ident ssorted_w\<iota>_stream cong: stream.map_cong)
+  subgoal for \<sigma>
+    apply safe
+    subgoal
+      apply (clarsimp simp: sincreasing_def ts_of_w_def)
+      subgoal for i
+        apply (insert w\<tau>_increasing[of "LEAST j. w\<iota>_stream \<sigma> !! i = w\<iota> \<sigma> j" \<sigma>])
+        apply clarify
+        subgoal for j
+          apply (insert sincreasing_w\<iota>_stream[THEN sincreasing_ex_greater, of "Suc i" "w\<iota> \<sigma> j" \<sigma>])
+          apply (clarsimp simp: Suc_le_eq)
+          subgoal for k
+            apply (rule exI[where x=k])
+            apply simp
+            apply (subgoal_tac "w\<tau> \<sigma> j \<le> w\<tau> \<sigma> (LEAST j. w\<iota>_stream \<sigma> !! k = w\<iota> \<sigma> j)")
+             apply (erule (1) order.strict_trans2)
+            apply (rule le_w\<iota>_le_w\<tau>)
+            by (metis (mono_tags, lifting) LeastI_ex ex_snth_w\<iota>_stream le_less_linear less_not_sym)
+          done
+        done
+      done
+    subgoal for i j
+      apply (erule mono_ts_of_w)
+       apply (rule ex_snth_w\<iota>_stream)+
+      done
+    done
+  done
+
+lemma wpartition_split: "wpartition n \<le> partition n \<circ>\<then> mapM_set relax_order"
+  apply (clarsimp simp: le_fun_def kleisli_set_def partition_def)
+  subgoal for \<sigma> ps
+    apply (rule exI[where x="map reorder_w ps"])
+    apply (auto simp: wpartition_def wtrace_partition_def
+        itrace_partition_def in_mapM_set_iff relax_order_def relaxed_order_def)
+    sorry (* TODO *)
+  done
+
+
+lemma length_islice[simp]: "length (islice f xs \<sigma>) = length xs"
+  by (simp add: islice_def)
+
+lemma in_partition_lengthD: "ps \<in> partition n \<sigma> \<Longrightarrow> length ps = n \<and> n > 0"
+  by (simp add: partition_def itrace_partition_def)
+
+lemma foldr_const_max: "foldr (\<lambda>x. max c) xs (a::_::linorder) = (if xs = [] then a else max c a)"
+  by (induction xs) simp_all
+
+lemma i\<tau>_islice[simp]: "k < length xs \<Longrightarrow> i\<tau> (islice f xs \<sigma> ! k) j = i\<tau> \<sigma> j"
+  by (simp add: islice_def)
+
+lemma i\<iota>_islice[simp]: "k < length xs \<Longrightarrow> i\<iota> (islice f xs \<sigma> ! k) j = i\<iota> \<sigma> j"
+  by (simp add: islice_def)
+
+lemma i\<Gamma>_islice[simp]: "k < length xs \<Longrightarrow> i\<Gamma> (islice f xs \<sigma> ! k) j = f (xs ! k) (i\<Gamma> \<sigma> j)"
+  by (simp add: islice_def)
+
+lemma partition_islice_transpose:
+  "partition n \<circ>\<then> determ (map (islice (\<inter>) xs)) \<circ>\<then> determ transpose \<le>
+    islice (\<inter>) xs \<circ>> mapM_set (partition n)"
+  apply (clarsimp simp: le_fun_def kleisli_set_def in_mapM_set_iff)
+  apply (rule list_all2_all_nthI)
+  subgoal 1 for \<sigma> ps
+    apply (subgoal_tac "ps \<noteq> []")
+     apply (simp add: length_transpose foldr_map foldr_const_max cong: foldr_cong)
+    apply (drule in_partition_lengthD)
+    apply clarsimp
+    done
+  subgoal for \<sigma> ps k
+    apply (frule 1)
+    apply (simp add: nth_transpose cong: map_cong)
+    apply (auto simp: partition_def itrace_partition_def cong: conj_cong)
+    by (meson le_infI2)
+  done
+
+notepad
+begin
+  fix add_index :: "'a trace \<Rightarrow> 'a itrace"
+  fix n :: nat
+  fix f :: "'b \<Rightarrow> 'a set"
+  fix xs :: "'a set list"
+
+  let ?p = "add_index \<circ>> wpartition n \<circ>\<then> determ (map (wslice (\<inter>) xs)) \<circ>\<then>
+    determ transpose \<circ>\<then> mapM_set linearize \<circ>\<then> determ (map reorder')"
+
+  have "?p \<le> add_index \<circ>> partition n \<circ>\<then> mapM_set relax_order \<circ>\<then> determ (map (wslice (\<inter>) xs)) \<circ>\<then>
+    determ transpose \<circ>\<then> mapM_set linearize \<circ>\<then> determ (map reorder')"
+    unfolding determ_kleisli_set[symmetric]
+    by (subst (5) kleisli_set_assoc) (intro kleisli_set_mono order_refl wpartition_split)
+  also have "\<dots> \<le> add_index \<circ>> partition n \<circ>\<then> determ (map (islice (\<inter>) xs)) \<circ>\<then> mapM_set (mapM_set relax_order) \<circ>\<then>
+    determ transpose \<circ>\<then> mapM_set linearize \<circ>\<then> determ (map reorder')"
+  proof -
+    have "mapM_set relax_order \<circ>\<then> determ (map (wslice (\<inter>) xs)) \<le> determ (map (islice (\<inter>) xs)) \<circ>\<then> mapM_set (mapM_set relax_order)"
+      by (auto simp: mapM_set_determ[symmetric] kleisli_mapM_set determ_kleisli_set
+        intro!: mapM_set_mono relax_order_wslice)
+    then show ?thesis
+      by (subst (1 5) kleisli_set_assoc) (intro kleisli_set_mono order_refl)
+  qed
+  also have "\<dots> \<le> add_index \<circ>> partition n \<circ>\<then> determ (map (islice (\<inter>) xs)) \<circ>\<then> determ transpose \<circ>\<then>
+    mapM_set (mapM_set relax_order) \<circ>\<then> mapM_set linearize \<circ>\<then> determ (map reorder')"
+    by (subst (2 6) kleisli_set_assoc) (auto simp: determ_kleisli_set
+      intro: kleisli_set_mono mapM_mapM_transpose)
+  also have "\<dots> \<le> add_index \<circ>> islice (\<inter>) xs \<circ>> mapM_set (partition n) \<circ>\<then>
+    mapM_set (mapM_set relax_order) \<circ>\<then> mapM_set linearize \<circ>\<then> determ (map reorder')"
+    unfolding fcomp_assoc unfolding determ_kleisli_set[symmetric]
+    apply (subst (1 2) kleisli_set_assoc)
+    apply (subst (2) kleisli_set_assoc[symmetric])
+    apply (intro kleisli_set_mono order_refl)
+    apply (simp add: determ_kleisli_set)
+    apply (rule partition_islice_transpose)
+    done
+end
 
 end
